move big int realted methods

RSAE3.dfy
@@ -1,368 +1,13 @@
 include "NativeTypes.dfy"
 include "Powers.dfy"
 include "Congruences.dfy"
+include "SeqInt.dfy"
 
 module RSAE3 {
     import opened NativeTypes
     import opened Powers
     import opened Congruences
-
-    const BASE :int := UINT32_MAX as int + 1;
-
-    function method reinterpret_cast(a: int64) : uint64
-
-    // |A[..n]| == n, interp A[..n] as an int 
-    function interp(A: seq<uint32>, n: nat) : nat
-        decreases n;
-        requires 0 <= n <= |A|;
-    {
-        if n == 0 then 0
-        else word_interp(A, n - 1) + interp(A, n - 1)
-    }
-
-    function R(n: nat) : nat
-        ensures R(n) != 0;
-    {
-        reveal power();
-        power(BASE, n)
-    }
-
-    function word_interp(A: seq<uint32>, i: nat) : nat
-        requires i < |A|;
-    {
-        A[i] as nat * postional_weight(i)
-    }
-
-    function postional_weight(i: nat) : nat
-    {
-        power(BASE, i) as nat
-    }
-
-    lemma {:induction i} word_interp_upper_bound_lemma(A: seq<uint32>, i: nat)
-        requires i < |A|;
-        ensures word_interp(A, i) <= power(BASE, i + 1) - power(BASE, i);
-    {
-        assert A[i] as int <= BASE;
-        calc ==> {
-            A[i] as int <= BASE;
-            A[i] as int * postional_weight(i) <= (BASE - 1) * postional_weight(i);
-            {
-                assert word_interp(A, i) == A[i] as int * postional_weight(i);
-            }
-             word_interp(A, i) <= (BASE - 1) * postional_weight(i);
-             word_interp(A, i) <= (BASE - 1) * power(BASE, i);
-             word_interp(A, i) <= BASE * power(BASE, i) - power(BASE, i);
-             {
-                power_add_one_lemma(BASE, i);
-             }
-             word_interp(A, i) <= power(BASE, i + 1) - power(BASE, i);
-        }
-    }
-
-    function seq_interp(A: seq<uint32>) : nat
-    {
-        interp(A, |A|)
-    }
-
-    lemma {:induction A} seq_interp_upper_bound_lemma(A: seq<uint32>, n: nat)
-        requires |A| == n != 0;
-        ensures seq_interp(A) < R(n);
-    {
-        if |A| == 1 {
-            reveal power();
-        } else {
-            ghost var A' := A[..(|A| - 1)];
-
-            calc ==> {
-                seq_interp(A) == word_interp(A, |A| - 1) + interp(A, |A| - 1);
-                {
-                    assert seq_interp(A') == interp(A, |A| - 1) by {
-                        prefix_sum_lemma(A, A', |A| - 1);
-                    }   
-                }
-                seq_interp(A) == word_interp(A, |A| - 1) + seq_interp(A');
-                {
-                    assert seq_interp(A') < power(BASE, |A'|);
-                }
-                seq_interp(A) < word_interp(A, |A| - 1) + power(BASE, |A'|);
-                {
-                    assert word_interp(A, |A| - 1) <= power(BASE, |A|) - power(BASE, |A| - 1) by {
-                        word_interp_upper_bound_lemma(A, |A| - 1);
-                    }
-                }
-                seq_interp(A) < power(BASE, |A|) - power(BASE, |A| - 1) + power(BASE, |A'|);
-                seq_interp(A) < power(BASE, |A|);
-            }
-        }
-    }
-
-    lemma postional_shift_lemma(i: int)
-        requires i > 0;
-        ensures postional_weight(i - 1) * BASE == postional_weight(i);
-    {
-        calc == {
-            postional_weight(i - 1) * BASE;
-            ==
-            power(BASE, i - 1) * BASE;
-            {
-                power_add_one_lemma(BASE, i - 1);
-            }
-            power(BASE, i);
-            ==
-            postional_weight(i);
-        }
-    }
-
-    lemma {:induction i} prefix_sum_lemma(S: seq<uint32>, S': seq<uint32>, i: nat)
-        requires 0 <= i <= |S| && 0 <= i <= |S'|;
-        requires S[..i] == S'[..i];
-        ensures interp(S, i) == interp(S', i);
-    {
-        assert true;
-    }
-
-    method seq_add_impl(A: seq<uint32>, B: seq<uint32>, n: nat) returns (c: uint2, S:seq<uint32>)
-        requires |A| == |B| == n;
-        ensures |S| == n;
-        ensures seq_interp(A) + seq_interp(B) == seq_interp(S) + c as int * postional_weight(n);
-        ensures n != 0 ==> cong(S[0] as int, A[0] as int + B[0] as int, BASE);
-    {
-        var temp := new uint32[|A|];
-        c, S := 0, temp[..];
-
-        var i: nat := 0;
-        ghost var S_old;
-
-        while i < n
-            invariant |S| == |A|;
-            invariant 0 <= i <= |A|;
-            decreases |A| - i;
-            invariant interp(A, i) + interp(B, i) == interp(S, i) + c as int * postional_weight(i);
-            invariant i > 0 ==> cong(S[0] as int, A[0] as int + B[0] as int, BASE);
-        {
-            ghost var c_old, i_old: int := c, i;
-            assert interp(A, i_old) + interp(B, i_old) == interp(S, i_old) + c_old as int * postional_weight(i_old);
-
-            var sum: uint64 := A[i] as uint64 + B[i] as uint64 + c as uint64;
-            var masked := and64(sum, UINT32_MAX as uint64) as uint32;
-            assume masked as int + BASE == sum as int;
-
-            S_old := S;
-            ghost var prefix_sum := interp(S_old, i);
-            S := S[i := masked];
-
-            if i == 0 {
-                assert cong(S[0] as int, A[0] as int + B[0] as int, BASE);
-            } else {
-                assert S[0] == S_old[0];
-            }
-
-            assert prefix_sum == interp(S, i_old) by {
-                prefix_sum_lemma(S, S_old, i_old);
-                assert interp(S, i_old) == interp(S_old, i_old);
-            }
-
-            i := i + 1;
-
-            assert interp(A, i_old) + interp(B, i_old) == interp(S, i_old) + c_old as int * postional_weight(i_old);
-            assert interp(S, i) == masked as int * postional_weight(i_old) + interp(S, i_old);
-            assert interp(B, i) == B[i - 1] as int * postional_weight(i - 1) + interp(B, i - 1);
-            assert interp(A, i) == A[i - 1] as int * postional_weight(i - 1) + interp(A, i - 1);
-
-            calc == {
-                interp(A, i) + interp(B, i);
-                ==
-                A[i - 1] as int * postional_weight(i - 1) + interp(A, i_old) +
-                B[i - 1] as int * postional_weight(i - 1) + interp(B, i_old);
-                ==
-                A[i - 1] as int * postional_weight(i - 1) + 
-                B[i - 1] as int * postional_weight(i - 1) +
-                interp(S, i_old) + c_old as int * postional_weight(i_old);
-                ==
-                postional_weight(i - 1) * (A[i - 1] as int + B[i - 1] as int + c_old as int) +
-                interp(S, i_old);
-                ==
-                postional_weight(i - 1) * (sum as int) + interp(S, i_old);
-            }
-
-            if sum > UINT32_MAX as uint64 {
-                c := 1;
-                calc == {
-                    postional_weight(i - 1) * (sum as int) + interp(S, i_old);
-                    postional_weight(i - 1) * masked as int + postional_weight(i - 1) * BASE + interp(S, i_old);
-                    {
-                        postional_shift_lemma(i);
-                    }
-                    postional_weight(i - 1) * masked as int + postional_weight(i) + interp(S, i_old);
-                }
-            } else {
-                c := 0;
-            }
-            assert interp(A, i) + interp(B, i) == interp(S, i) + c as int * postional_weight(i);
-        }
-    }
-
-    method seq_add(A: seq<uint32>, B: seq<uint32>, n: nat) returns (S: seq<uint32>)
-        requires |A| == |B| == n;
-        ensures |S| == n;
-        ensures cong(seq_interp(A) + seq_interp(B), seq_interp(S), power(BASE, n));
-        ensures n != 0 ==> cong(S[0] as int, A[0] as int + B[0] as int, BASE);
-    {
-        var c;
-        c, S := seq_add_impl(A, B, n);
-
-        if c == 0 {
-            assert cong(seq_interp(A) + seq_interp(B), seq_interp(S), power(BASE, n)) by {
-                assert seq_interp(A) + seq_interp(B) == seq_interp(S);
-                reveal cong();
-            }
-        } else {
-            assert cong(seq_interp(A) + seq_interp(B), seq_interp(S), power(BASE, n)) by {
-                assert cong(seq_interp(A) + seq_interp(B), seq_interp(S) + postional_weight(n), power(BASE, n)) by {
-                    assert seq_interp(A) + seq_interp(B) == seq_interp(S) + postional_weight(n);
-                    reveal cong();
-                }
-                assert cong(seq_interp(S) + power(BASE, n), seq_interp(S), power(BASE, n)) by {
-                    cong_add_lemma_3(seq_interp(S), power(BASE, n), power(BASE, n));
-                    reveal cong();
-                }
-                cong_trans_lemma(seq_interp(A) + seq_interp(B), seq_interp(S) + power(BASE, n), seq_interp(S), power(BASE, n));
-            }
-        }
-    }
-
-    method seq_add_c(A: seq<uint32>, B: seq<uint32>, n: nat) returns (S: seq<uint32>)
-        requires |A| == |B| == n;
-        ensures |S| == n + 1;
-        ensures seq_interp(A) + seq_interp(B) == seq_interp(S)
-        ensures n != 0 ==> cong(S[0] as int, A[0] as int + B[0] as int, BASE);
-    {
-        var c, S' := seq_add_impl(A, B, n);
-        S := S' + [c as uint32];
-        calc == {
-            seq_interp(A) + seq_interp(B);
-            seq_interp(S') + c as int * postional_weight(n);
-            seq_interp(S') + word_interp(S, n);
-            interp(S', n) + word_interp(S, n);
-            {
-                prefix_sum_lemma(S, S', n);
-            }
-            interp(S, n) + word_interp(S, n);
-            seq_interp(S);
-        }
-    }
-
-    lemma {:induction m} zero_extend_lemma(A: seq<uint32>, n: nat, A': seq<uint32>, m: nat)
-        requires |A| == n && |A'| == m;
-        requires n < m;
-        requires forall i :: 0 <= i < n ==> A[i] == A'[i];
-        requires forall i :: n <= i < m ==> A'[i] == 0;
-        ensures seq_interp(A') == seq_interp(A); 
-    {
-        if m != n {
-            assume false;
-        }
-    }
-
-    method seq_zero_extend(A: seq<uint32>, n: nat, m: nat) returns (A': seq<uint32>)
-        requires |A| == n;
-        requires m > n;
-        ensures |A'| == m;
-        ensures seq_interp(A') == seq_interp(A); 
-        ensures forall i :: 0 <= i < n ==> A[i] == A'[i];
-        ensures forall i :: n <= i < m ==> A'[i] == 0;
-    {
-        var temp := new uint32[m];
-        var i := 0;
-
-        while i < m 
-            decreases m - i;
-            invariant forall j:: 0 <= j < i < n ==> temp[j] == A[j];
-            invariant forall j:: n <=  j < i < m ==> temp[j] == 0;
-        {
-            if i < n {
-                temp[i] := A[i];
-            } else {
-                temp[i] := 0;
-            }
-            i := i + 1;
-        }
-
-        assume false;
-        A' := temp[..];
-    }
-
-    method seq_sub(A: seq<uint32>, B: seq<uint32>) returns (b: uint2, S:seq<uint32>)
-        requires |A| == |B|;
-        ensures seq_interp(A) - seq_interp(B) == seq_interp(S) - b as int * postional_weight(|A|);
-    {
-        var temp := new uint32[|A|];
-        b, S := 0, temp[..];
-
-        var i: nat := 0;
-
-        while i < |A|
-            invariant |S| == |A|;
-            invariant 0 <= i <= |A|;
-            decreases |A| - i;
-            invariant interp(A, i) - interp(B, i) == interp(S, i) - b as int * postional_weight(i);
-        {
-            var b_old, i_old: int := b, i;
-            assert interp(A, i_old) - interp(B, i_old) == interp(S, i_old) - b_old as int * postional_weight(i_old);
-
-            var diff: int64 := A[i] as int64 - B[i] as int64 - b as int64;
-            var masked := and64(reinterpret_cast(diff), UINT32_MAX as uint64) as uint32;
-
-            assume diff < 0 ==> masked as int == diff as int + BASE as int;
-            assume diff >= 0 ==> masked as int == diff as int;
-
-            ghost var S_old := S;
-            ghost var prefix_sum := interp(S_old, i);
-            S := S[i := masked];
-
-            assert prefix_sum == interp(S, i_old) by {
-                prefix_sum_lemma(S, S_old, i_old);
-                assert interp(S, i_old) == interp(S_old, i_old);
-            }
-
-            i := i + 1;
-
-            assert interp(A, i_old) - interp(B, i_old) == interp(S, i_old) - b_old as int * postional_weight(i_old);
-            assert interp(S, i) == masked as int * postional_weight(i_old) + interp(S, i_old);
-            assert interp(B, i) == B[i - 1] as int * postional_weight(i - 1) + interp(B, i - 1);
-            assert interp(A, i) == A[i - 1] as int * postional_weight(i - 1) + interp(A, i - 1);
-
-            calc == {
-                interp(A, i) - interp(B, i);
-                ==
-                A[i - 1] as int * postional_weight(i - 1) + interp(A, i_old) -
-                B[i - 1] as int * postional_weight(i - 1) - interp(B, i_old);
-                ==
-                A[i - 1] as int * postional_weight(i - 1) - 
-                B[i - 1] as int * postional_weight(i - 1) +
-                interp(S, i_old) - b_old as int * postional_weight(i_old);
-                ==
-                postional_weight(i - 1) * (A[i - 1] as int - B[i - 1] as int - b_old as int) +
-                interp(S, i_old);
-            }
-
-            if diff < 0 {
-                b := 1;
-                calc == {
-                    postional_weight(i - 1) * (diff as int) + interp(S, i_old);
-                    postional_weight(i - 1) * masked as int - postional_weight(i - 1) * BASE + interp(S, i_old);
-                    {
-                        postional_shift_lemma(i);
-                    }
-                    postional_weight(i - 1) * masked as int - postional_weight(i) + interp(S, i_old);
-                }
-            } else {                
-                b := 0;
-                assert interp(A, i) - interp(B, i) == interp(S, i);
-            }
-            assert interp(A, i) - interp(B, i) == interp(S, i) - b as int * postional_weight(i);
-        }
-    }
+    import opened SeqInt
 
     lemma mont_mul_div_aux_lemma_2(y: int, x: int, m: int, a: int, m': int)
         requires cong(m' * m, -1, BASE);
@@ -805,11 +450,16 @@ module RSAE3 {
         assume seq_interp(A) == 0;
         var i := 0;
 
+        assert seq_interp(A) == (seq_interp(x[..i]) * seq_interp(y) / power(BASE, i)) % seq_interp(m);
+
         while i < n
             decreases n - i;
             invariant |A| == n + 1;
             invariant seq_interp(A) < 2 * seq_interp(m) - 1;
+            // invariant seq_interp(A) == (seq_interp(x[..i]) * seq_interp(y) * power(BASE_INV, i)) % seq_interp(m);
         {
+            assume seq_interp(A) == (seq_interp(x[..i]) * seq_interp(y) / power(BASE, i)) % seq_interp(m);
+
             var u_i_ := ((A[0] as int + x[i] as int * y[0] as int) * m' as int) % BASE; 
             var u_i := u_i_ as uint32;
 
@@ -823,12 +473,18 @@ module RSAE3 {
                 mont_mul_divisible_lemma(m, x, y, P_1, P_2, S, A, A', i, u_i, m', n);
             }
         
+            calc ==> {
+
+            }
+
             assert seq_interp(A'[1..n+2]) < 2 * seq_interp(m) - 1 by {
                 mont_mul_bound_lemma(m, x, y, P_1, P_2, S, A, A', i, u_i, m', n);
             }
 
-            A := A'[1..n+2];
+            var A'' := A'[1..n+2];
+
             i := i + 1;
+            A := A'';
         }
     }
 
